F_mu_ref_par/fundamental_binary.v
@@ -4,121 +4,96 @@ From iris_logrel.F_mu_ref_par Require Import rules_binary.
 From iris.algebra Require Export upred_big_op.
 
 Section typed_interp.
-  Context {Σ : gFunctors} {iI : heapIG Σ} {iS : cfgSG Σ} {N : namespace}.
-  Implicit Types Δ : varC -n> bivalC -n> iPropG lang Σ.
-  Implicit Types P Q R : iPropG lang Σ.
+  Context `{heapIG Σ, cfgSG Σ} (N : namespace).
+  Notation D := (prodC valC valC -n> iPropG lang Σ).
+  Implicit Types e : expr.
+  Implicit Types Δ : listC D.
+  Hint Resolve to_of_val.
 
   Local Tactic Notation "smart_wp_bind" uconstr(ctx) ident(v) ident(w)
         constr(Hv) uconstr(Hp) :=
     iApply (@wp_bind _ _ _ [ctx]);
     iApply wp_wand_l; iSplitR;
-    [|iApply Hp; rewrite fill_app; simpl; repeat iSplitR; trivial];
+    [|iApply Hp; rewrite ?fill_app; simpl; repeat iSplitR; trivial];
     let Htmp := iFresh in
     iIntros {v} Htmp; iDestruct Htmp as {w} Hv;
     rewrite fill_app; simpl.
 
   Local Ltac value_case := iApply wp_value; [cbn; rewrite ?to_of_val; trivial|].
 
-  Lemma map_lookup {A B} (l : list A) (f : A → B) k :
-    map f l !! k = option_map f (l !! k).
-  Proof.
-    revert k; induction l => k; simpl; trivial.
-    destruct k; simpl; trivial.
-  Qed.
-
-  Definition bin_log_related Δ Γ e e' τ {HΔ : ∀ x vw, PersistentP (Δ x vw)} :=
-    ∀ vs, length Γ = length vs →
-    ∀ ρ j K,
-      heapI_ctx (N .@ 2) ★ Spec_ctx (N .@ 3) ρ ★
-        [∧] zip_with (λ τ, interp (N .@ 1) τ Δ) Γ vs ★
-        j ⤇ fill K (e'.[env_subst (map snd vs)])
-      ⊢ WP e.[env_subst (map fst vs)] {{ v, ∃ v',
-          j ⤇ fill K (# v') ★ interp (N .@ 1) τ Δ (v, v') }}.
+  Definition bin_log_related (Δ : listC D) (Γ : list type)
+      (e e' : expr) (τ : type) : Prop := ∀ vvs ρ j K,
+    length Γ = length vvs →
+    heapI_ctx (N .@ 2) ★ Spec_ctx (N .@ 3) ρ ★
+      [∧] zip_with (λ τ, interp (N .@ 1) τ Δ) Γ vvs ★
+      j ⤇ fill K (e'.[env_subst (map snd vvs)])
+    ⊢ WP e.[env_subst (vvs.*1)] {{ v, ∃ v',
+        j ⤇ fill K (# v') ★ interp (N .@ 1) τ Δ (v, v') }}.
 
   Notation "Δ ∥ Γ ⊩ e '≤log≤' e' ∷ τ" := (bin_log_related Δ Γ e e' τ)
-                                       (at level 20) : bin_logrel_scope.
+                                       (at level 20).
 
-  Local Open Scope bin_logrel_scope.
-
-  Notation "✓✓ Δ" := (∀ x v, PersistentP (Δ x v)) (at level 20).
+  Notation "✓✓ Δ" := (ctx_PersistentP Δ) (at level 20).
 
   Lemma typed_binary_interp_Pair Δ Γ e1 e2 e1' e2' τ1 τ2 {HΔ : ✓✓ Δ}
       (IHHtyped1 : Δ ∥ Γ ⊩ e1 ≤log≤ e1' ∷ τ1)
       (IHHtyped2 : Δ ∥ Γ ⊩ e2 ≤log≤ e2' ∷ τ2) :
     Δ ∥ Γ ⊩ Pair e1 e2 ≤log≤ Pair e1' e2' ∷ TProd τ1 τ2.
   Proof.
-    iIntros {vs Hlen ρ j K} "(#Hheap & #Hspec & #HΓ & Htr) /=".
-    smart_wp_bind (PairLCtx e2.[env_subst (map fst vs)]) v v' "[Hv #Hiv]"
-                  (IHHtyped1 _ _ _ j
-                             (K ++ [PairLCtx e2'.[env_subst (map snd vs)] ])).
+    iIntros {vvs ρ j K Hlen} "(#Hh & #Hs & #HΓ & Hj) /=".
+    smart_wp_bind (PairLCtx e2.[env_subst _]) v v' "[Hv #Hiv]"
+      (IHHtyped1 _ _ j (K ++ [PairLCtx e2'.[env_subst _] ])).
     smart_wp_bind (PairRCtx v) w w' "[Hw #Hiw]"
-                  (IHHtyped2 _ _ _ j (K ++ [(PairRCtx v')])).
+      (IHHtyped2 _ _ j (K ++ [PairRCtx v'])).
     value_case. iExists (PairV v' w'); iFrame "Hw".
-    iExists (v, w), (v', w'); simpl; repeat iSplit; trivial.
-    (* unshelving *)
-    Unshelve. all: trivial.
+    iExists (v, v'), (w, w'); simpl; repeat iSplit; trivial.
   Qed.
 
   Lemma typed_binary_interp_Fst Δ Γ e e' τ1 τ2 {HΔ : ✓✓ Δ}
       (IHHtyped : Δ ∥ Γ ⊩ e ≤log≤ e' ∷ TProd τ1 τ2) :
     Δ ∥ Γ ⊩ Fst e ≤log≤ Fst e' ∷ τ1.
   Proof.
-    iIntros {vs Hlen ρ j K} "(#Hheap & #Hspec & #HΓ & Htr)"; cbn.
-    smart_wp_bind (FstCtx) v v' "[Hv #Hiv]"
-                  (IHHtyped _ _ _ j (K ++ [FstCtx])); cbn.
-    iDestruct "Hiv" as {w1 w2} "#[% [Hiv2 Hiv3]]"; simplify_eq.
-    iPvs (step_fst _ _ _ j K (# (w2.1)) (w2.1) (# (w2.2)) (w2.2)
-                   _ _ _ with "* [-]") as "Hw".
-    iFrame "Hspec Hv"; trivial.
-    iApply wp_fst; try iPvsIntro; eauto using to_of_val; cbn.
-    (* unshelving *)
-    Unshelve. all: eauto using to_of_val.
+    iIntros {vvs ρ j K Hlen} "(#Hh & #Hs & #HΓ & Hj) /=".
+    smart_wp_bind (FstCtx) v v' "[Hv #Hiv]" (IHHtyped _ _ j (K ++ [FstCtx])); cbn.
+    iDestruct "Hiv" as { [w1 w1'] [w2 w2'] } "#[% [Hw1 Hw2]]"; simplify_eq.
+    iPvs (step_fst (N .@ 3) _ _ j K (# w1') w1' (# w2') w2' with "* [-]") as "Hw"; eauto.
+    iApply wp_fst; eauto.
   Qed.
 
   Lemma typed_binary_interp_Snd Δ Γ e e' τ1 τ2 {HΔ : ✓✓ Δ}
       (IHHtyped : Δ ∥ Γ ⊩ e ≤log≤ e' ∷ TProd τ1 τ2) :
     Δ ∥ Γ ⊩ Snd e ≤log≤ Snd e' ∷ τ2.
   Proof.
-    iIntros {vs Hlen ρ j K} "(#Hheap & #Hspec & #HΓ & Htr)"; cbn.
-    smart_wp_bind (SndCtx) v v' "[Hv #Hiv]"
-                  (IHHtyped _ _ _ j (K ++ [SndCtx])); cbn.
-    iDestruct "Hiv" as {w1 w2} "#[% [Hiv2 Hiv3]]"; simplify_eq.
-    iPvs (step_snd _ _ _ j K (# (w2.1)) (w2.1) (# (w2.2)) (w2.2)
-                   _ _ _ with "* [-]") as "Hw".
-    iFrame "Hspec Hv"; trivial.
-    iApply wp_snd; eauto using to_of_val; cbn.
-    (* unshelving *)
-    Unshelve. all: eauto using to_of_val.
+    iIntros {vvs ρ j K Hlen} "(#Hh & #Hs & #HΓ & Hj) /=".
+    smart_wp_bind (SndCtx) v v' "[Hv #Hiv]" (IHHtyped _ _ j (K ++ [SndCtx])); cbn.
+    iDestruct "Hiv" as { [w1 w1'] [w2 w2'] } "#[% [Hw1 Hw2]]"; simplify_eq.
+    iPvs (step_snd (N .@ 3) _ _ j K (# w1') w1' (# w2') w2' with "* [-]") as "Hw"; eauto.
+    iApply wp_snd; eauto.
   Qed.
 
   Lemma typed_binary_interp_InjL Δ Γ e e' τ1 τ2 {HΔ : ✓✓ Δ}
       (IHHtyped : Δ ∥ Γ ⊩ e ≤log≤ e' ∷ τ1) :
     Δ ∥ Γ ⊩ InjL e ≤log≤ InjL e' ∷ (TSum τ1 τ2).
   Proof.
-    iIntros {vs Hlen ρ j K} "(#Hheap & #Hspec & #HΓ & Htr)"; cbn.
+    iIntros {vvs ρ j K Hlen} "(#Hh & #Hs & #HΓ & Hj) /=".
     smart_wp_bind (InjLCtx) v v' "[Hv #Hiv]"
-                  (IHHtyped _ _ _ j (K ++ [InjLCtx])); cbn.
+      (IHHtyped _ _ j (K ++ [InjLCtx])); cbn.
     value_case. iExists (InjLV v'); iFrame "Hv".
-    iLeft; iExists _; iSplit; [|eauto]; simpl; trivial.
-    (* unshelving *)
-    Unshelve. all: trivial.
+    iLeft; iExists (_,_); eauto 10.
   Qed.
 
   Lemma typed_binary_interp_InjR Δ Γ e e' τ1 τ2 {HΔ : ✓✓ Δ}
       (IHHtyped : Δ ∥ Γ ⊩ e ≤log≤ e' ∷ τ2) :
     Δ ∥ Γ ⊩ InjR e ≤log≤ InjR e' ∷ TSum τ1 τ2.
   Proof.
-    intros vs Hlen ρ j K. iIntros "(#Hheap & #Hspec & #HΓ & Htr)"; cbn.
+    iIntros {vvs ρ j K Hlen} "(#Hh & #Hs & #HΓ & Hj) /=".
     smart_wp_bind (InjRCtx) v v' "[Hv #Hiv]"
-                  (IHHtyped _ _ _ j (K ++ [InjRCtx])); cbn.
+      (IHHtyped _ _ j (K ++ [InjRCtx])); cbn.
     value_case. iExists (InjRV v'); iFrame "Hv".
-    iRight; iExists _; iSplit; [|eauto]; simpl; trivial.
-    (* unshelving *)
-    Unshelve. all: trivial.
+    iRight; iExists (_,_); eauto 10.
   Qed.
 
-  Lemma typed_binary_interp_Case Δ Γ (e0 e1 e2 e0' e1' e2' : expr) τ1 τ2 τ3
-      {HΔ : ✓✓ Δ}
+  Lemma typed_binary_interp_Case Δ Γ e0 e1 e2 e0' e1' e2' τ1 τ2 τ3 {HΔ : ✓✓ Δ}
       (Hclosed2 : ∀ f, e1.[iter (S (length Γ)) up f] = e1)
       (Hclosed3 : ∀ f, e2.[iter (S (length Γ)) up f] = e2)
       (Hclosed2' : ∀ f, e1'.[iter (S (length Γ)) up f] = e1')
@@ -128,31 +103,24 @@ Section typed_interp.
       (IHHtyped3 : Δ ∥ τ2 :: Γ ⊩ e2 ≤log≤ e2' ∷ τ3) :
     Δ ∥ Γ ⊩ Case e0 e1 e2 ≤log≤ Case e0' e1' e2' ∷ τ3.
   Proof.
-    iIntros {vs Hlen ρ j K} "(#Hheap & #Hspec & #HΓ & Htr) /=".
+    iIntros {vvs ρ j K Hlen} "(#Hh & #Hs & #HΓ & Hj) /=".
     smart_wp_bind (CaseCtx _ _) v v' "[Hv #Hiv]"
-                  (IHHtyped1 _ _ _ j (K ++ [CaseCtx _ _])); cbn.
+      (IHHtyped1 _ _ j (K ++ [CaseCtx _ _])); cbn.
     iDestruct "Hiv" as "[Hiv|Hiv]".
-    + iDestruct "Hiv" as {w} "[% Hw]"; simplify_eq.
-      iPvs (step_case_inl _ _ _ j K (# (w.2)) (w.2) _ _
-                          _ _ with "* [-]") as "Hz".
-      iFrame "Hspec Hv"; trivial.
-      iApply wp_case_inl; auto 1 using to_of_val.
-      asimpl.
-      specialize (IHHtyped2 (w::vs)); simpl in IHHtyped2.
+    - iDestruct "Hiv" as { [w w'] } "[% Hw]"; simplify_eq.
+      iPvs (step_case_inl (N .@ 3) _ _ j K (# w') w' with "* [-]") as "Hz"; eauto.
+      iApply wp_case_inl; auto 1 using to_of_val; asimpl.
+      specialize (IHHtyped2 ((w,w') :: vvs)); cbn in IHHtyped2.
       erewrite <- ?n_closed_subst_head_simpl in IHHtyped2; eauto;
-        simpl; try rewrite map_length; eauto with f_equal. iNext.
-      iApply IHHtyped2; eauto.
-    + iDestruct "Hiv" as {w} "[% Hw]"; simplify_eq.
-      iPvs (step_case_inr _ _ _ j K (# (w.2)) (w.2) _ _ _ _ with "* [-]") as "Hz".
-      iFrame "Hspec Hv"; trivial.
-      iApply wp_case_inr; auto 1 using to_of_val.
-      asimpl.
-      specialize (IHHtyped3 (w::vs)); simpl in IHHtyped3.
+        simpl; try rewrite fmap_length; eauto with f_equal.
+      iNext. iApply IHHtyped2; eauto.
+    - iDestruct "Hiv" as { [w w'] } "[% Hw]"; simplify_eq.
+      iPvs (step_case_inr (N .@ 3) _ _ j K (# w') w' with "* [-]") as "Hz"; eauto.
+      iApply wp_case_inr; auto 1 using to_of_val; asimpl.
+      specialize (IHHtyped3 ((w,w') :: vvs)); cbn in IHHtyped3.
       erewrite <- ?n_closed_subst_head_simpl in IHHtyped3; eauto;
-        simpl; try rewrite map_length; eauto with f_equal. iNext.
-      iApply IHHtyped3; eauto 10.
-      (* unshelving *)
-      Unshelve. all: eauto using to_of_val.
+        simpl; try rewrite map_length; eauto with f_equal.
+      iNext. iApply IHHtyped3; eauto 10.
   Qed.
 
   Lemma typed_binary_interp_If Δ Γ e0 e1 e2 e0' e1' e2' τ {HΔ : ✓✓ Δ}
@@ -161,18 +129,14 @@ Section typed_interp.
       (IHHtyped3 : Δ ∥ Γ ⊩ e2 ≤log≤ e2' ∷ τ) :
     Δ ∥ Γ ⊩ If e0 e1 e2 ≤log≤ If e0' e1' e2' ∷ τ.
   Proof.
-    iIntros {vs Hlen ρ j K} "(#Hheap & #Hspec & #HΓ & Htr) /=".
+    iIntros {vvs ρ j K Hlen} "(#Hh & #Hs & #HΓ & Hj) /=".
     smart_wp_bind (IfCtx _ _) v v' "[Hv #Hiv]"
-                  (IHHtyped1 _ _ _ j (K ++ [IfCtx _ _])); cbn.
+      (IHHtyped1 _ _ j (K ++ [IfCtx _ _])); cbn.
     iDestruct "Hiv" as { [] } "[% %]"; simplify_eq/=.
-    + iPvs (step_if_true _ _ _ j K _ _ _ with "* [-]") as "Hz".
-      iFrame "Hspec Hv"; trivial. iApply wp_if_true. iNext.
-      iApply IHHtyped2; eauto.
-    + iPvs (step_if_false _ _ _ j K _ _ _ with "* [-]") as "Hz".
-      iFrame "Hspec Hv"; trivial. iApply wp_if_false. iNext.
-      iApply IHHtyped3; eauto.
-      (* unshelving *)
-      Unshelve. all: eauto using to_of_val.
+    - iPvs (step_if_true (N .@ 3) _ _ j K with "* [-]") as "Hz"; eauto.
+      iApply wp_if_true. iNext. iApply IHHtyped2; eauto.
+    - iPvs (step_if_false (N .@ 3) _ _ j K with "* [-]") as "Hz"; eauto.
+      iApply wp_if_false. iNext. iApply IHHtyped3; eauto.
   Qed.
 
   Lemma typed_binary_interp_nat_bin_op Δ Γ op e1 e2 e1' e2' {HΔ : ✓✓ Δ}
@@ -180,20 +144,17 @@ Section typed_interp.
       (IHHtyped2 : Δ ∥ Γ ⊩ e2 ≤log≤ e2' ∷ TNat) :
     Δ ∥ Γ ⊩ BinOp op e1 e2 ≤log≤ BinOp op e1' e2' ∷ binop_res_type op.
   Proof.
-    iIntros {vs Hlen ρ j K} "(#Hheap & #Hspec & #HΓ & Htr)"; cbn.
+    iIntros {vvs ρ j K Hlen} "(#Hh & #Hs & #HΓ & Hj) /=".
     smart_wp_bind (BinOpLCtx _ _) v v' "[Hv #Hiv]"
-                  (IHHtyped1 _ _ _ j (K ++ [BinOpLCtx _ _])); cbn.
+                  (IHHtyped1 _ _ j (K ++ [BinOpLCtx _ _])); cbn.
     smart_wp_bind (BinOpRCtx _ _) w w' "[Hw #Hiw]"
-                  (IHHtyped2 _ _ _ j (K ++ [BinOpRCtx _ _])); cbn.
-    iDestruct "Hiv" as {n} "[% %]"; subst; simpl.
-    iDestruct "Hiw" as {n'} "[% %]"; subst; simpl.
-    iPvs (step_nat_bin_op _ _ _ j K _ _ _ _ with "* [-]") as "Hz".
-    iFrame "Hspec Hw"; trivial. iApply wp_nat_bin_op. iNext. iPvsIntro.
-    iExists _; iSplitL; eauto.
+                  (IHHtyped2 _ _ j (K ++ [BinOpRCtx _ _])); cbn.
+    iDestruct "Hiv" as {n} "[% %]"; simplify_eq/=.
+    iDestruct "Hiw" as {n'} "[% %]"; simplify_eq/=.
+    iPvs (step_nat_bin_op (N .@ 3) _ _ j K with "* [-]") as "Hz"; eauto.
+    iApply wp_nat_bin_op. iNext. iPvsIntro. iExists _; iSplitL; eauto.
     destruct op; simpl; try destruct eq_nat_dec; try destruct le_dec;
-      try destruct lt_dec; iExists _; iSplit; trivial.
-    (* unshelving *)
-    Unshelve. all: eauto using to_of_val.
+      try destruct lt_dec; eauto.
   Qed.
 
   Lemma typed_binary_interp_Lam Δ Γ (e e' : expr) τ1 τ2 {HΔ : ✓✓ Δ}
@@ -202,21 +163,17 @@ Section typed_interp.
       (IHHtyped : Δ ∥ TArrow τ1 τ2 :: τ1 :: Γ ⊩ e ≤log≤ e' ∷ τ2) :
     Δ ∥ Γ ⊩ Lam e ≤log≤ Lam e' ∷ TArrow τ1 τ2.
   Proof.
-    iIntros {vs Hlen ρ j K} "(#Hheap & #Hspec & #HΓ & Htr) /=".
-    value_case. iExists (LamV _). iFrame "Htr". iAlways.
-    iLöb as "IH". iIntros {j' K' v} "[#Hiv Hv]".
+    iIntros {vvs ρ j K Hlen} "(#Hh & #Hs & #HΓ & Hj) /=".
+    value_case. iExists (LamV _). iIntros "{$Hj} !".
+    iLöb as "IH". iIntros {j' K' [v v'] } "[#Hiv Hv]".
     iApply wp_lam; auto 1 using to_of_val. iNext.
-    iPvs (step_lam _ _ _ j' K' _ (# (v.2)) (v.2) _ _ with "* [-]") as "Hz".
-    iFrame "Hspec Hv"; trivial.
+    iPvs (step_lam (N .@ 3) _ _ j' K' _ (# v') v' with "* [-]") as "Hz"; eauto.
     asimpl.
-    specialize (IHHtyped ((LamV e.[upn 2 (env_subst (map fst vs))],
-                           LamV e'.[upn 2 (env_subst (map snd vs))])
-                            :: v :: vs)). simpl in IHHtyped.
+    specialize (IHHtyped ((LamV e.[upn 2 (env_subst (vvs.*1))],
+      LamV e'.[upn 2 (env_subst (vvs.*2))]) :: (v,v') :: vvs)); cbn in IHHtyped.
     erewrite <- ?n_closed_subst_head_simpl_2 in IHHtyped; eauto; simpl;
-      try rewrite map_length; auto.
+      try rewrite fmap_length; auto.
     iApply IHHtyped; eauto 10.
-    (* unshelving *)
-    Unshelve. all: eauto using to_of_val.
   Qed.
 
   Lemma typed_binary_interp_App Δ Γ e1 e2 e1' e2' τ1 τ2 {HΔ : ✓✓ Δ}
@@ -224,145 +181,116 @@ Section typed_interp.
       (IHHtyped2 : Δ ∥ Γ ⊩ e2 ≤log≤ e2' ∷ τ1) :
     Δ ∥ Γ ⊩ App e1 e2 ≤log≤ App e1' e2' ∷  τ2.
   Proof.
-    iIntros {vs Hlen ρ j K} "(#Hheap & #Hspec & #HΓ & Htr) /=".
-    smart_wp_bind (AppLCtx (e2.[env_subst (map fst vs)])) v v' "[Hv #Hiv]"
-                  (IHHtyped1 _ _ _ j
-                     (K ++ [(AppLCtx (e2'.[env_subst (map snd vs)]))])); cbn.
+    iIntros {vvs ρ j K Hlen} "(#Hh & #Hs & #HΓ & Hj) /=".
+    smart_wp_bind (AppLCtx (e2.[env_subst (vvs.*1)])) v v' "[Hv #Hiv]"
+      (IHHtyped1 _ _ j (K ++ [(AppLCtx (e2'.[env_subst (vvs.*2)]))])); cbn.
     smart_wp_bind (AppRCtx v) w w' "[Hw #Hiw]"
-                  (IHHtyped2 _ _ _ j (K ++ [AppRCtx v'])); cbn.
+      (IHHtyped2 _ _ j (K ++ [AppRCtx v'])); cbn.
     iApply ("Hiv" $! j K (w, w')); simpl; eauto.
-    (* unshelving *)
-    Unshelve. all: trivial.
   Qed.
 
   Lemma typed_binary_interp_TLam Δ Γ e e' τ {HΔ : ✓✓ Δ}
-      (IHHtyped : ∀ (τi : bivalC -n> _) (Hpr: ∀ vw, PersistentP (τi vw)),
-      (extend_context_interp_fun1 τi Δ) ∥ map (λ t : type, t.[ren (+1)]) Γ
-                                        ⊩ e ≤log≤ e' ∷ τ) :
+      (IHHtyped : ∀ (τi : D), (∀ vw, PersistentP (τi vw)) →
+      (τi :: Δ) ∥ (subst (ren (+1)) <$> Γ) ⊩ e ≤log≤ e' ∷ τ) :
     Δ ∥ Γ ⊩ TLam e ≤log≤ TLam e' ∷ TForall τ.
   Proof.
-    iIntros {vs Hlen ρ j K} "(#Hheap & #Hspec & #HΓ & Htr) /=".
-    value_case. iExists (TLamV _). iFrame "Htr"; simpl.
-    iAlways; iIntros {τi j' K'} "% Hv /=".
+    iIntros {vvs ρ j K Hlen} "(#Hh & #Hs & #HΓ & Hj) /=".
+    value_case. iExists (TLamV _).
+    iIntros "{$Hj} /= !"; iIntros {τi j' K'} "% Hv /=".
     iApply wp_TLam; iNext.
-    iPvs (step_Tlam _ _ _ j' K' (e'.[env_subst (map snd vs)]) _ with "* [-]")
-      as "Hz".
-    iFrame "Hspec Hv"; trivial.
-    iApply IHHtyped; [rewrite map_length; trivial|].
-    iFrame "Hheap Hspec".
-    rewrite zip_with_context_interp_subst; by iFrame "HΓ".
-    Unshelve. all: trivial.
+    iPvs (step_Tlam (N .@ 3) _ _ j' K' (e'.[env_subst (vvs.*2)]) with "* [-]")
+      as "Hz"; eauto.
+    iApply IHHtyped; [by rewrite fmap_length|].
+    iFrame "Hh Hs Hz". rewrite zip_with_fmap_l. by iApply context_interp_ren_S.
   Qed.
 
   Lemma typed_binary_interp_TApp Δ Γ e e' τ τ' {HΔ : ✓✓ Δ}
       (IHHtyped : Δ ∥ Γ ⊩ e ≤log≤ e' ∷ TForall τ) :
     Δ ∥ Γ ⊩ TApp e ≤log≤ TApp e' ∷ τ.[τ'/].
   Proof.
-    iIntros {vs Hlen ρ j K} "(#Hheap & #Hspec & #HΓ & Htr) /=".
+    iIntros {vvs ρ j K Hlen} "(#Hh & #Hs & #HΓ & Hj) /=".
     smart_wp_bind (TAppCtx) v v' "[Hj #Hv]"
-                    (IHHtyped _ _ _ j (K ++ [TAppCtx])); cbn.
+      (IHHtyped _ _ j (K ++ [TAppCtx])); cbn.
     iApply wp_wand_r; iSplitL.
     { iApply ("Hv" $! (interp (N .@ 1) τ' Δ) with "[#] Hj"); iPureIntro; apply _. }
     iIntros {w} "Hw". iDestruct "Hw" as {w'} "[Hw #Hiw]".
     iExists _; rewrite -interp_subst; eauto.
-    (* unshelving *)
-    Unshelve. all: trivial.
   Qed.
 
   Lemma typed_binary_interp_Fold Δ Γ e e' τ {HΔ : ✓✓ Δ}
       (IHHtyped : Δ ∥ Γ ⊩ e ≤log≤ e' ∷ τ.[(TRec τ)/]) :
     Δ ∥ Γ ⊩ Fold e ≤log≤ Fold e' ∷ TRec τ.
   Proof.
-    iIntros {vs Hlen ρ j K} "(#Hheap & #Hspec & #HΓ & Htr) /=".
+    iIntros {vvs ρ j K Hlen} "(#Hh & #Hs & #HΓ & Hj) /=".
     iApply (@wp_bind _ _ _ [FoldCtx]);
       iApply wp_wand_l; iSplitR;
-        [|iApply (IHHtyped _ _ _ j (K ++ [FoldCtx]));
-          rewrite fill_app; simpl; repeat iSplitR; trivial].
-    iIntros {v} "Hv"; iDestruct "Hv" as {w} "[Hv #Hiv]";
-      rewrite fill_app.
+        [|iApply (IHHtyped _ _ j (K ++ [FoldCtx]));
+          rewrite ?fill_app; simpl; repeat iSplitR; trivial].
+    iIntros {v}; iDestruct 1 as {w} "[Hv #Hiv]"; rewrite fill_app.
     value_case. iExists (FoldV w); iFrame "Hv".
-    rewrite fixpoint_unfold; cbn.
-    rewrite -interp_subst; trivial.
+    rewrite fixpoint_unfold /= -interp_subst.
     iAlways; iExists (_, _); eauto.
-    (* unshelving *)
-    Unshelve. all: trivial.
   Qed.
 
   Lemma typed_binary_interp_Unfold Δ Γ e e' τ {HΔ : ✓✓ Δ}
       (IHHtyped : Δ ∥ Γ ⊩ e ≤log≤ e' ∷ TRec τ) :
     Δ ∥ Γ ⊩ Unfold e ≤log≤ Unfold e' ∷ τ.[(TRec τ)/].
   Proof.
-    iIntros {vs Hlen ρ j K} "(#Hheap & #Hspec & #HΓ & Htr) /=".
+    iIntros {vvs ρ j K Hlen} "(#Hh & #Hs & #HΓ & Hj) /=".
     iApply (@wp_bind _ _ _ [UnfoldCtx]);
       iApply wp_wand_l; iSplitR;
-        [|iApply (IHHtyped _ _ _ j (K ++ [UnfoldCtx]));
-          rewrite fill_app; simpl; repeat iSplitR; trivial].
-    iIntros {v} "Hv". iDestruct "Hv" as {w} "[Hw #Hiw]"; rewrite fill_app.
-    simpl. rewrite fixpoint_unfold; simpl.
+        [|iApply (IHHtyped _ _ j (K ++ [UnfoldCtx]));
+          rewrite ?fill_app; simpl; repeat iSplitR; trivial].
+    iIntros {v}. iDestruct 1 as {v'} "[Hw #Hiw]"; rewrite fill_app.
+    rewrite /= fixpoint_unfold /=.
     change (fixpoint _) with (@interp _ _ _ (N .@ 1) (TRec τ) Δ).
-    iDestruct "Hiw" as {z} "#[% Hiz]"; simplify_eq/=.
-    iPvs (step_Fold _ _ _ j K (# (z.2)) (z.2) _ _ with "* [-]") as "Hz".
-    iFrame "Hspec Hw"; trivial.
-    iApply wp_Fold; cbn; auto using to_of_val.
-    iNext. iExists _; iFrame "Hz".
-    rewrite -interp_subst; destruct z; trivial.
-    (* unshelving *)
-    Unshelve. all: eauto using to_of_val.
+    iDestruct "Hiw" as { [w w'] } "#[% Hiz]"; simplify_eq/=.
+    iPvs (step_Fold _ _ _ j K (# w') w' with "* [-]") as "Hz"; eauto.
+    iApply wp_Fold; cbn; auto.
+    iNext; iPvsIntro; iExists _; iFrame "Hz". by rewrite -interp_subst.
   Qed.
 
   Lemma typed_binary_interp_Fork Δ Γ e e' {HΔ : ✓✓ Δ}
       (IHHtyped : Δ ∥ Γ ⊩ e ≤log≤ e' ∷ TUnit) :
     Δ ∥ Γ ⊩ Fork e ≤log≤ Fork e' ∷ TUnit.
   Proof.
-    iIntros {vs Hlen ρ j K} "(#Hheap & #Hspec & #HΓ & Htr) /=".
-    iPvs (step_fork _ _ _ j K _ _ with "* [-]") as {j'} "[Hz1 Hz2]"; first by iFrame.
-    iApply wp_fork; iNext; iSplitL "Hz1".
-    + iExists UnitV; iFrame "Hz1"; eauto.
-    + iApply wp_wand_l; iSplitR; [|iApply (IHHtyped _ _ _ _ [])]; eauto.
-    (* unshelving *)
-    Unshelve. all: trivial.
+    iIntros {vvs ρ j K Hlen} "(#Hh & #Hs & #HΓ & Hj) /=".
+    iPvs (step_fork (N .@ 3) _ _ j K with "* [-]") as {j'} "[Hj Hj']"; eauto.
+    iApply wp_fork; iNext; iSplitL "Hj".
+    - iExists UnitV; eauto.
+    - iApply wp_wand_l; iSplitR; [|iApply (IHHtyped _ _ _ [])]; eauto.
   Qed.
 
   Lemma typed_binary_interp_Alloc Δ Γ e e' τ {HΔ : ✓✓ Δ}
       (IHHtyped : Δ ∥ Γ ⊩ e ≤log≤ e' ∷ τ) :
     Δ ∥ Γ ⊩ Alloc e ≤log≤ Alloc e' ∷ Tref τ.
   Proof.
-    iIntros {vs Hlen ρ j K} "(#Hheap & #Hspec & #HΓ & Htr) /=".
-    smart_wp_bind (AllocCtx) v v' "[Hv #Hiv]"
-                  (IHHtyped _ _ _ j (K ++ [AllocCtx])).
-    iPvs (step_alloc _ _ _ j K (# v') v' _ _ with "* [-]") as {l'} "[Hj Hl']"; eauto.
-    iApply wp_alloc; auto 1 using to_of_val.
-    iIntros "{$Hheap} >". iIntros {l} "Hl".
-    iAssert ((∃ w : val * val, l ↦ᵢ w.1 ★ l' ↦ₛ w.2 ★
-                                 ((@interp _ _ _ (N .@ 1) τ) Δ) w)%I)
-      with "[Hl Hl']" as "Hinv".
-    { iExists (v, v'); iFrame "Hl Hl' Hiv"; trivial. }
-    iPvs (inv_alloc _ with "[Hinv]") as "HN"; eauto 1.
-    { iNext; iExact "Hinv". }
-    iPvsIntro. iExists (LocV l'); iSplit; [iExact "Hj"|].
-    iExists (l, l'); iSplit; trivial.
-    (* unshelving *)
-    Unshelve. all: eauto using to_of_val.
+    iIntros {vvs ρ j K Hlen} "(#Hh & #Hs & #HΓ & Hj) /=".
+    smart_wp_bind (AllocCtx) v v' "[Hv #Hiv]" (IHHtyped _ _ j (K ++ [AllocCtx])).
+    iPvs (step_alloc (N .@ 3) _ _ j K (# v') v' with "* [-]") as {l'} "[Hj Hl]"; eauto.
+    iApply wp_alloc; auto.
+    iIntros "{$Hh} >"; iIntros {l} "Hl'".
+    iPvs (inv_alloc (N .@ 1 .@ (l,l')) _ (∃ w : val * val,
+      l ↦ᵢ w.1 ★ l' ↦ₛ w.2 ★ interp (N .@ 1) τ Δ w)%I with "[Hl Hl']") as "HN"; eauto.
+    { iNext; iExists (v, v'); by iFrame. }
+    iPvsIntro; iExists (LocV l'). iFrame "Hj". iExists (l, l'); eauto.
   Qed.
 
   Lemma typed_binary_interp_Load Δ Γ e e' τ {HΔ : ✓✓ Δ}
       (IHHtyped : Δ ∥ Γ ⊩ e ≤log≤ e' ∷ (Tref τ)) :
     Δ ∥ Γ ⊩ Load e ≤log≤ Load e' ∷ τ.
   Proof.
-    iIntros {vs Hlen ρ j K} "(#Hheap & #Hspec & #HΓ & Htr) /=".
-    smart_wp_bind (LoadCtx) v v' "[Hv #Hiv]"
-                  (IHHtyped _ _ _ j (K ++ [LoadCtx])).
-    iDestruct "Hiv" as {l} "[% Hinv]"; simplify_eq/=.
-    iInv (N .@ 1 .@ l) as {w} "[Hw1 [Hw2 #Hw3]]".
+    iIntros {vvs ρ j K Hlen} "(#Hh & #Hs & #HΓ & Hj) /=".
+    smart_wp_bind (LoadCtx) v v' "[Hv #Hiv]" (IHHtyped _ _ j (K ++ [LoadCtx])).
+    iDestruct "Hiv" as { [l l'] } "[% Hinv]"; simplify_eq/=.
+    iInv (N .@ 1 .@ (l,l')) as { [w w'] } "[Hw1 [Hw2 #Hw]]"; simpl.
     iTimeless "Hw2".
-    iPvs (step_load _ _ _ j K (l.2) 1 (w.2) _ with "[Hv Hw2]") as "[Hv Hw2]".
-    iFrame "Hspec Hv"; trivial.
-    iApply (wp_load _ _ _ 1); [|iFrame "Hheap"]; trivial. solve_ndisj.
+    iPvs (step_load (N .@ 3) _ _ j K l' 1 w' with "[Hv Hw2]") as "[Hv Hw2]";
+      [solve_ndisj|by iFrame|].
+    iApply (wp_load _ _ _ 1); [|iFrame "Hh"]; trivial; try solve_ndisj.
     iIntros "{$Hw1} > Hw1". iPvsIntro. iSplitL "Hw1 Hw2".
-    + iNext; iExists w; by iFrame.
-    + destruct w as [w1 w2]; iExists w2; iFrame "Hv Hw3"; trivial.
-      (* unshelving *)
-      Unshelve. all: eauto using to_of_val || solve_ndisj.
+    - iNext; iExists (w,w'); by iFrame.
+    - iExists w'; by iFrame.
   Qed.
 
   Lemma typed_binary_interp_Store Δ Γ e1 e2 e1' e2' τ {HΔ : ✓✓ Δ}
@@ -370,24 +298,21 @@ Section typed_interp.
       (IHHtyped2 : Δ ∥ Γ ⊩ e2 ≤log≤ e2' ∷ τ) :
     Δ ∥ Γ ⊩ Store e1 e2 ≤log≤ Store e1' e2' ∷ TUnit.
   Proof.
-    iIntros {vs Hlen ρ j K} "(#Hheap & #Hspec & #HΓ & Htr) /=".
+    iIntros {vvs ρ j K Hlen} "(#Hh & #Hs & #HΓ & Hj) /=".
     smart_wp_bind (StoreLCtx _) v v' "[Hv #Hiv]"
-                  (IHHtyped1 _ _ _ j (K ++ [StoreLCtx _])).
+      (IHHtyped1 _ _ j (K ++ [StoreLCtx _])).
     smart_wp_bind (StoreRCtx _) w w' "[Hw #Hiw]"
-                  (IHHtyped2 _ _ _ j (K ++ [StoreRCtx _])).
-    iDestruct "Hiv" as {l} "[% Hinv]"; simplify_eq/=.
-    iInv (N .@ 1 .@ l) as {z} "[Hw1 [Hw2 #Hw3]]".
-    eapply bool_decide_spec; eauto using to_of_val.
-    iTimeless "Hw2".
-    iPvs (step_store _ _ _ j K (l.2) (z.2) (# w') w' _ _ with "[Hw Hw2]")
-      as "[Hw Hw2]".
-    iFrame "Hspec Hw Hw2"; trivial.
+      (IHHtyped2 _ _ j (K ++ [StoreRCtx _])).
+    iDestruct "Hiv" as { [l l'] } "[% Hinv]"; simplify_eq/=.
+    iInv (N .@ 1 .@ (l,l')) as { [v v'] } "[Hv1 [Hv2 #Hv]]".
+    { eapply bool_decide_spec; eauto using to_of_val. }
+    iTimeless "Hv2".
+    iPvs (step_store (N .@ 3) _ _ j K l' v' (# w') w' with "[Hw Hv2]")
+      as "[Hw Hv2]"; [eauto|solve_ndisj|by iFrame|].
     iApply (wp_store (N .@ 2)); auto using to_of_val. solve_ndisj.
-    iIntros "{$Hheap $Hw1} > Hw1". iPvsIntro. iSplitL "Hw1 Hw2".
-    + iNext; iExists (w, w'); by iFrame.
-    + iExists UnitV; iFrame "Hw" ; iSplit; trivial.
-      (* unshelving *)
-      Unshelve. all: eauto using to_of_val || solve_ndisj.
+    iIntros "{$Hh $Hv1} > Hv1". iPvsIntro. iSplitL "Hv1 Hv2".
+    - iNext; iExists (w, w'); by iFrame.
+    - iExists UnitV; iFrame; auto.
   Qed.
 
   Lemma typed_binary_interp_CAS Δ Γ e1 e2 e3 e1' e2' e3' τ {HΔ : ✓✓ Δ}
@@ -397,84 +322,77 @@ Section typed_interp.
       (IHHtyped3 : Δ ∥ Γ ⊩ e3 ≤log≤ e3' ∷ τ) :
     Δ ∥ Γ ⊩ CAS e1 e2 e3 ≤log≤ CAS e1' e2' e3' ∷ TBool.
   Proof.
-    iIntros {vs Hlen ρ j K} "(#Hheap & #Hspec & #HΓ & Htr) /=".
+    iIntros {vvs ρ j K Hlen} "(#Hh & #Hs & #HΓ & Hj) /=".
     smart_wp_bind (CasLCtx _ _) v v' "[Hv #Hiv]"
-                  (IHHtyped1 _ _ _ j (K ++ [CasLCtx _ _])).
+      (IHHtyped1 _ _ j (K ++ [CasLCtx _ _])).
     smart_wp_bind (CasMCtx _ _) w w' "[Hw #Hiw]"
-                  (IHHtyped2 _ _ _ j (K ++ [CasMCtx _ _])).
+      (IHHtyped2 _ _ j (K ++ [CasMCtx _ _])).
     smart_wp_bind (CasRCtx _ _) u u' "[Hu #Hiu]"
-                  (IHHtyped3 _ _ _ j (K ++ [CasRCtx _ _])).
-    iDestruct "Hiv" as {l} "[% Hinv]"; simplify_eq/=.
-    iInv (N .@ 1 .@ l) as { [z1 z2] } "[Hw1 [Hw2 #Hw3]]".
-    eapply bool_decide_spec; eauto 10 using to_of_val.
-    iTimeless "Hw2".
-    destruct (val_dec_eq z1 w) as [|Hneq]; subst.
-    + iPvs (step_cas_suc _ _ _ j K (l.2) (# w') w' z2 (# u') u' _ _ _
-            with "[Hu Hw2]") as "[Hw Hw2]"; simpl.
-      { iFrame "Hspec Hu Hw2". iNext.
-        rewrite ?EqType_related_eq; trivial.
-        iDestruct "Hiw" as "%". iDestruct "Hw3" as "%".
-        repeat subst; trivial. }
-      iApply (wp_cas_suc (N .@ 2)); eauto using to_of_val. solve_ndisj.
-      iIntros "{$Hheap $Hw1} > Hw1". iPvsIntro. iSplitL "Hw1 Hw2".
-      * iNext; iExists (_, _); iFrame "Hw1 Hw2"; trivial.
-      * iExists (♭v true); iFrame "Hw"; eauto.
-    + iPvs (step_cas_fail _ _ _ j K (l.2) 1 (z2) (# w') w' (# u') u' _ _ _
-            with "[Hu Hw2]") as "[Hw Hw2]"; simpl.
-      { iFrame "Hspec Hu Hw2". iNext.
-        rewrite ?EqType_related_eq; trivial.
-        iDestruct "Hiw" as "%". iDestruct "Hw3" as "%"; subst; eauto. }
-      iApply (wp_cas_fail (N .@ 2)); eauto using to_of_val. solve_ndisj.
-      iIntros "{$Hheap $Hw1} > Hw1". iPvsIntro. iSplitL "Hw1 Hw2".
-      * iNext; iExists (_, _); by iFrame "Hw1 Hw2".
-      * iExists (♭v false); eauto.
-        (* unshelving *)
-        Unshelve. all: eauto using to_of_val || solve_ndisj.
+      (IHHtyped3 _ _ j (K ++ [CasRCtx _ _])).
+    iDestruct "Hiv" as { [l l'] } "[% Hinv]"; simplify_eq/=.
+    iInv (N .@ 1 .@ (l,l')) as { [v v'] } "[Hv1 [Hv2 #Hv]]".
+    { eapply bool_decide_spec; eauto 10 using to_of_val. }
+    iTimeless "Hv2".
+    destruct (decide (v = w)) as [|Hneq]; subst.
+    - iPvs (step_cas_suc (N .@ 3) _ _ j K l' (# w') w' v' (# u') u'
+            with "[Hu Hv2]") as "[Hw Hv2]"; simpl; eauto; first solve_ndisj.
+      { iIntros "{$Hs $Hu $Hv2} >".
+        rewrite ?interp_EqType_agree; trivial. by iSimplifyEq. }
+      iApply (wp_cas_suc (N .@ 2)); eauto using to_of_val; first solve_ndisj.
+      iIntros "{$Hh $Hv1} > Hv1". iPvsIntro. iSplitL "Hv1 Hv2".
+      + iNext; iExists (_, _); by iFrame.
+      + iExists (♭v true); iFrame; eauto.
+    - iPvs (step_cas_fail (N .@ 3) _ _ j K l' 1 v' (# w') w' (# u') u'
+            with "[Hu Hv2]") as "[Hw Hv2]"; simpl; eauto; first solve_ndisj.
+      { iIntros "{$Hs $Hu $Hv2} >".
+        rewrite ?interp_EqType_agree; trivial. by iSimplifyEq. }
+      iApply (wp_cas_fail (N .@ 2)); eauto using to_of_val; first solve_ndisj.
+      iIntros "{$Hh $Hv1} > Hv1". iPvsIntro. iSplitL "Hv1 Hv2".
+      + iNext; iExists (_, _); by iFrame.
+      + iExists (♭v false); eauto.
   Qed.
 
-  Lemma typed_binary_interp Δ Γ e τ {HΔ : ∀ x vw, PersistentP (Δ x vw)} :
+  Lemma typed_binary_interp Δ Γ e τ {HΔ : ctx_PersistentP Δ} :
     Γ ⊢ₜ e : τ → Δ ∥ Γ ⊩ e ≤log≤ e ∷ τ.
   Proof.
     intros Htyped; revert Δ HΔ; induction Htyped; intros Δ HΔ.
-    - iIntros {vs Hlen ρ j K} "(#Hheap & #Hspec & #HΓ & Htr) /=".
-      destruct (lookup_lt_is_Some_2 vs x) as [v Hv].
+    - iIntros {vvs ρ j K Hlen} "(#Hh & #Hs & #HΓ & Hj) /=".
+      destruct (lookup_lt_is_Some_2 vvs x) as [[v v'] Hv].
       { by rewrite -Hlen; apply lookup_lt_Some with τ. }
-      rewrite /env_subst. repeat rewrite map_lookup. rewrite Hv; simpl.
-      value_case.
-      iExists _; iFrame "Htr".
+      rewrite /env_subst !list_lookup_fmap Hv /=. value_case.
+      iExists _; iFrame "Hj".
       iApply (big_and_elem_of with "HΓ").
       apply elem_of_list_lookup_2 with x.
-      rewrite lookup_zip_with; simplify_option_eq; destruct v; trivial.
-    - iIntros {vs Hlen ρ j K} "(#Hheap & #Hspec & #HΓ & Htr) /=".
+      rewrite lookup_zip_with; by simplify_option_eq.
+    - iIntros {vvs ρ j K Hlen} "(#Hh & #Hs & #HΓ & Hj) /=".
       value_case. iExists UnitV; eauto.
-    - iIntros {vs Hlen ρ j K} "(#Hheap & #Hspec & #HΓ & Htr) /=".
+    - iIntros {vvs ρ j K Hlen} "(#Hh & #Hs & #HΓ & Hj) /=".
       value_case. iExists (♯v _); eauto.
-    - iIntros {vs Hlen ρ j K} "(#Hheap & #Hspec & #HΓ & Htr) /=".
+    - iIntros {vvs ρ j K Hlen} "(#Hh & #Hs & #HΓ & Hj) /=".
       value_case. iExists (♭v _); eauto.
-    - apply typed_binary_interp_nat_bin_op; trivial.
-    - apply typed_binary_interp_Pair; trivial.
-    - eapply typed_binary_interp_Fst; trivial.
-    - eapply typed_binary_interp_Snd; trivial.
-    - eapply typed_binary_interp_InjL; trivial.
-    - eapply typed_binary_interp_InjR; trivial.
+    - apply typed_binary_interp_nat_bin_op; eauto.
+    - apply typed_binary_interp_Pair; eauto.
+    - eapply typed_binary_interp_Fst; eauto.
+    - eapply typed_binary_interp_Snd; eauto.
+    - eapply typed_binary_interp_InjL; eauto.
+    - eapply typed_binary_interp_InjR; eauto.
     - eapply typed_binary_interp_Case; eauto;
         match goal with H : _ |- _ => eapply (typed_n_closed _ _ _ H) end.
     - eapply typed_binary_interp_If; eauto.
     - eapply typed_binary_interp_Lam; eauto;
         match goal with H : _ |- _ => eapply (typed_n_closed _ _ _ H) end.
-    - eapply typed_binary_interp_App; trivial.
-    - eapply typed_binary_interp_TLam; trivial.
-    - eapply typed_binary_interp_TApp; trivial.
-    - eapply typed_binary_interp_Fold; trivial.
-    - eapply typed_binary_interp_Unfold; trivial.
-    - eapply typed_binary_interp_Fork; trivial.
-    - eapply typed_binary_interp_Alloc; trivial.
-    - eapply typed_binary_interp_Load; trivial.
-    - eapply typed_binary_interp_Store; trivial.
+    - eapply typed_binary_interp_App; eauto.
+    - eapply typed_binary_interp_TLam; eauto with typeclass_instances.
+    - eapply typed_binary_interp_TApp; eauto.
+    - eapply typed_binary_interp_Fold; eauto.
+    - eapply typed_binary_interp_Unfold; eauto.
+    - eapply typed_binary_interp_Fork; eauto.
+    - eapply typed_binary_interp_Alloc; eauto.
+    - eapply typed_binary_interp_Load; eauto.
+    - eapply typed_binary_interp_Store; eauto.
     - eapply typed_binary_interp_CAS; eauto.
   Qed.
 End typed_interp.
 
-Notation "Δ ∥ Γ ⊩ e '≤log≤' e' ∷ τ" := (bin_log_related Δ Γ e e' τ)
-                                         (at level 20) : bin_logrel_scope.
-Delimit Scope bin_logrel_scope with bin_logrel.
+Notation "Δ ∥ Γ ⊩ e '≤log≤' e' ∷ τ" :=
+  (bin_log_related Δ Γ e e' τ) (at level 20).
