F_mu_ref_par/logrel_binary.v
@@ -3,460 +3,203 @@ From iris.program_logic Require Export weakestpre.
 From iris_logrel.F_mu_ref_par Require Export rules_binary typing.
 Import uPred.
 
+(* HACK: move somewhere else *)
+Ltac auto_proper ::=
+  (* Deal with "pointwise_relation" *)
+  repeat lazymatch goal with
+  | |- pointwise_relation _ _ _ _ => intros ?
+  end;
+  (* Normalize away equalities. *)
+  repeat match goal with
+  | H : _ ≡{_}≡ _ |-  _ => apply (timeless_iff _ _) in H
+  | _ => progress simplify_eq
+  end;
+  (* repeatedly apply congruence lemmas and use the equalities in the hypotheses. *)
+  try (f_equiv; fast_done || auto_proper).
+
 (** interp : is a unary logical relation. *)
 Section logrel.
-  Context {Σ : gFunctors}.
+  Context `{heapIG Σ, cfgSG Σ} (L : namespace).
+  Notation D := (prodC valC valC -n> iPropG lang Σ).
+  Implicit Types τi : D.
+  Implicit Types Δ : listC D.
+  Implicit Types interp : listC D → D.
 
-  Canonical Structure bivalC := prodC valC valC.
+  Program Definition ctx_lookup (x : var) : listC D -n> D := λne Δ,
+    from_option id (cconst True)%I (Δ !! x).
+  Solve Obligations with solve_proper_alt.
 
-  (** Just to get nicer closed forms, we define extend_context_interp in
-      three steps. *)
-  Program Definition extend_context_interp_fun1
-      (τi : bivalC -n> iPropG lang Σ)
-      (f : varC -n> bivalC -n> iPropG lang Σ) :
-      (varC -n> bivalC -n> iPropG lang Σ) := λne x,
-    match x return bivalC -n> iPropG lang Σ with O => τi | S x' => f x' end.
+  Program Definition interp_unit : listC D -n> D := λne Δ ww,
+    (ww.1 = UnitV ∧ ww.2 = UnitV)%I.
+  Solve Obligations with solve_proper_alt.
+  Program Definition interp_nat : listC D -n> D := λne Δ ww,
+    (∃ n : nat, ww.1 = ♯v n ∧ ww.2 = ♯v n)%I.
+  Solve Obligations with solve_proper.
+  Program Definition interp_bool : listC D -n> D := λne Δ ww,
+    (∃ b : bool, ww.1 = ♭v b ∧ ww.2 = ♭v b)%I.
+  Solve Obligations with solve_proper.
 
-  Program Definition extend_context_interp_fun2
-      (τi : bivalC -n> iPropG lang Σ) :
-      (varC -n> bivalC -n> iPropG lang Σ) -n>
-      (varC -n> bivalC -n> iPropG lang Σ) := λne f,
-    extend_context_interp_fun1 τi f.
-  Next Obligation. intros ???? Hfg x; destruct x; cbn; trivial. Qed.
+  Program Definition interp_prod
+      (interp1 interp2 : listC D -n> D) : listC D -n> D := λne Δ ww,
+    (∃ vv1 vv2, ww = (PairV (vv1.1) (vv2.1), PairV (vv1.2) (vv2.2)) ∧
+                interp1 Δ vv1 ∧ interp2 Δ vv2)%I.
+  Solve Obligations with solve_proper.
 
-  Program Definition extend_context_interp :
-      (bivalC -n> iPropG lang Σ) -n>
-      (varC -n> bivalC -n> iPropG lang Σ) -n>
-      (varC -n> bivalC -n> iPropG lang Σ) := λne τi,
-    extend_context_interp_fun2 τi.
-  Next Obligation. intros n g h H Δ x y. destruct x; cbn; auto. Qed.
+  Program Definition interp_sum
+      (interp1 interp2 : listC D -n> D) : listC D -n> D := λne Δ ww,
+    ((∃ vv, ww = (InjLV (vv.1), InjLV (vv.2)) ∧ interp1 Δ vv) ∨
+     (∃ vv, ww = (InjRV (vv.1), InjRV (vv.2)) ∧ interp2 Δ vv))%I.
+  Solve Obligations with solve_proper.
 
-  Program Definition extend_context_interp_apply :
-      ((varC -n> bivalC -n> iPropG lang Σ)) -n>
-      ((varC -n> bivalC -n> iPropG lang Σ) -n>
-       bivalC -n> iPropG lang Σ) -n>
-      (bivalC -n> iPropG lang Σ) -n> (bivalC -n> iPropG lang Σ) := λne Δ f g,
-    f (extend_context_interp g Δ).
-  Solve Obligations with
-  repeat intros ?; (cbn + idtac);
-    try match goal with [H : _ ≡{_}≡ _|- _] => rewrite H end; trivial.
+  Program Definition interp_arrow
+      (interp1 interp2 : listC D -n> D) : listC D -n> D := λne Δ ww,
+    (□ ∀ j K vv,
+      interp1 Δ vv ★ j ⤇ fill K (App (# ww.2) (# vv.2)) →
+      WP App (# ww.1) (# vv.1) {{ v, ∃ v', j ⤇ fill K (# v') ★ interp2 Δ (v, v') }})%I.
+  Solve Obligations with solve_proper.
+
+  Program Definition interp_forall
+      (interp : listC D -n> D) : listC D -n> D := λne Δ ww,
+    (□ ∀ τi j K,
+       (■ ∀ ww, PersistentP (τi ww)) →
+       j ⤇ fill K (TApp (# ww.2)) →
+       WP TApp (# ww.1) {{ v, ∃ v', j ⤇ fill K (# v') ★ interp (τi :: Δ) (v, v')}})%I.
+  Solve Obligations with solve_proper.
+
+  Program Definition interp_rec1
+      (interp : listC D -n> D) (Δ : listC D) (τi : D) : D := λne ww,
+    (□ ∃ vv, ww = (FoldV (vv.1), FoldV (vv.2)) ∧ ▷ interp (τi :: Δ) vv)%I.
+  Solve Obligations with solve_proper.
+
+  Global Instance interp_rec1_contractive
+    (interp : listC D -n> D) (Δ : listC D) : Contractive (interp_rec1 interp Δ).
+  Proof.
+    intros n τi1 τi2 Hτi ww; cbn.
+    apply always_ne, exist_ne; intros vv; apply and_ne; trivial.
+    apply later_contractive =>i Hi. by rewrite Hτi.
+  Qed.
+
+  Program Definition interp_rec (interp : listC D -n> D) : listC D -n> D := λne Δ,
+    fixpoint (interp_rec1 interp Δ).
   Next Obligation.
-    intros n Δ Δ' HΔ f g x.  cbn.
-    match goal with
-      |- _ _ ?F x ≡{n}≡ _ _ ?G x =>
-      assert (F ≡{n}≡ G) as HFG; [|rewrite HFG; trivial]
+    intros interp n Δ1 Δ2 HΔ; apply fixpoint_ne => τi ww. solve_proper.
+  Qed.
+
+  Program Definition interp_ref_inv (ll : loc * loc) : D -n> iPropG lang Σ := λne τi,
+    (∃ vv, ll.1 ↦ᵢ vv.1 ★ ll.2 ↦ₛ vv.2 ★ τi vv)%I.
+  Solve Obligations with solve_proper.
+
+  Program Definition interp_ref
+      (interp : listC D -n> D) : listC D -n> D := λne Δ ww,
+    (∃ ll, ww = (LocV (ll.1), LocV (ll.2)) ∧
+           inv (L .@ ll) (interp_ref_inv ll (interp Δ)))%I.
+  Solve Obligations with solve_proper.
+
+  Fixpoint interp (τ : type) : listC D -n> D :=
+    match τ return _ with
+    | TUnit => interp_unit
+    | TNat => interp_nat
+    | TBool => interp_bool
+    | TProd τ1 τ2 => interp_prod (interp τ1) (interp τ2)
+    | TSum τ1 τ2 => interp_sum (interp τ1) (interp τ2)
+    | TArrow τ1 τ2 => interp_arrow (interp τ1) (interp τ2)
+    | TVar x => ctx_lookup x
+    | TForall τ' => interp_forall (interp τ')
+    | TRec τ' => interp_rec (interp τ')
+    | Tref τ' => interp_ref (interp τ')
     end.
-    apply cofe_mor_car_ne; trivial. intros y. cbn.
-    destruct y; trivial.
-  Qed.
 
-  Program Definition interp_unit : bivalC -n> iPropG lang Σ := λne w,
-    (w.1 = UnitV ∧ w.2 = UnitV)%I.
-  Next Obligation. intros n x y [H1 H2]; rewrite H1 H2; trivial. Qed.
+  Class ctx_PersistentP Δ :=
+    ctx_persistentP : Forall (λ τi, ∀ vv, PersistentP (τi vv)) Δ.
+  Global Instance ctx_persistent_nil : ctx_PersistentP [].
+  Proof. by constructor. Qed.
+  Global Instance ctx_persistent_cons τi Δ :
+    (∀ vv, PersistentP (τi vv)) → ctx_PersistentP Δ → ctx_PersistentP (τi :: Δ).
+  Proof. by constructor. Qed.
+  Global Instance ctx_persistent_lookup Δ x vv :
+    ctx_PersistentP Δ → PersistentP (ctx_lookup x Δ vv).
+  Proof. intros HΔ; revert x; induction HΔ=>-[|?] /=; apply _. Qed.
 
-  Program Definition interp_nat : bivalC -n> iPropG lang Σ := λne w,
-    (∃ n, w.1 = (♯v n) ∧ w.2 = (♯v n))%I.
-  Next Obligation. intros n x y [H1 H2]; rewrite H1 H2; trivial. Qed.
-
-  Program Definition interp_bool : bivalC -n> iPropG lang Σ :=λne w,
-    (∃ b, w.1 = (♭v b) ∧ w.2 = (♭v b))%I.
-  Next Obligation. intros n x y [H1 H2]; rewrite H1 H2; trivial. Qed.
-
-  Program Definition interp_prod :
-      (bivalC -n> iPropG lang Σ) -n> (bivalC -n> iPropG lang Σ) -n>
-      bivalC -n> iPropG lang Σ := λne τ1i τ2i w,
-    (∃ w1 w2, w = (PairV (w1.1) (w1.2), PairV (w2.1) (w2.2)) ∧
-              τ1i (w1.1, w2.1) ∧ τ2i (w1.2, w2.2))%I.
-  Next Obligation.
-    intros τ1i τ2i n [x1 x2] [y1 y2] [H1 H2]; simpl in *.
-    rewrite H1 H2; trivial.
-  Qed.
-  Next Obligation. solve_proper. Qed.
-  Next Obligation. solve_proper. Qed.
-
-  Program Definition interp_sum :
-      (bivalC -n> iPropG lang Σ) -n> (bivalC -n> iPropG lang Σ) -n>
-      bivalC -n> iPropG lang Σ := λne τ1i τ2i w,
-    ((∃ w1, w = (InjLV (w1.1), InjLV (w1.2)) ∧ τ1i w1) ∨
-     (∃ w2, w = (InjRV (w2.1), InjRV (w2.2)) ∧ τ2i w2))%I.
-  Next Obligation.
-    intros τ1i τ2i n [x1 x2] [y1 y2] [H1 H2]; simpl in *.
-    rewrite H1 H2; trivial.
-  Qed.
-  Next Obligation. solve_proper. Qed.
-  Next Obligation. solve_proper. Qed.
-
-  Context `{Si : cfgSG Σ}.
-
-  Program Definition interp_arrow :
-      (bivalC -n> iPropG lang Σ) -n> (bivalC -n> iPropG lang Σ) -n>
-      bivalC -n> iPropG lang Σ := λne τ1i τ2i w,
-    (□ ∀ j K v,
-      τ1i v ★ j ⤇ (fill K (App (# w.2) (# v.2))) →
-      WP App (# w.1) (# v.1) {{ z, ∃ z', j ⤇ (fill K (# z')) ★ τ2i (z, z') }})%I.
-  Next Obligation. 
-    intros τ1i τ2i n [x1 x2] [y1 y2] [H1 H2]; simpl in *.
-    rewrite H1 H2; trivial.
-  Qed.
-  Next Obligation. solve_proper. Qed.
-  Next Obligation. solve_proper. Qed.
-
-  Program Definition interp_forall :
-      ((bivalC -n> iPropG lang Σ) -n> (bivalC -n> iPropG lang Σ)) -n>
-      bivalC -n> iPropG lang Σ := λne τi w,
-    (□ ∀ (f : bivalC -n> iPropG lang Σ) j K,
-       (■ (∀ vw, PersistentP (f vw))) →
-       j ⤇ (fill K (TApp (# w.2))) →
-       WP TApp (# w.1) {{ v, ∃ v', j ⤇ fill K (# v') ★ τi f (v, v')}})%I.
-  Next Obligation.
-    intros τi n [x1 x2] [y1 y2 ] [H1 H2]. simpl in *; auto.
-    inversion H1; subst; inversion H2; subst; trivial.
-  Qed.
-  Next Obligation. solve_proper. Qed.
-
-  Program Definition interp_rec_pre :
-      ((bivalC -n> iPropG lang Σ) -n> (bivalC -n> iPropG lang Σ)) -n>
-      (bivalC -n> iPropG lang Σ) -n>
-      (bivalC -n> iPropG lang Σ) := λne τi rec_appr w,
-    (□ (∃ v, w = (FoldV (v.1), FoldV (v.2)) ∧ ▷ (τi rec_appr v)))%I.
-  Next Obligation.
-    intros τi rec_appr n [x1 x2] [y1 y2] [H1 H2]; simpl in *.
-    inversion H1; inversion H2; subst; trivial.
-  Qed.
-  Next Obligation. solve_proper. Qed.
-  Next Obligation. solve_proper. Qed.
-
-  Global Instance interp_rec_pre_contr
-      (τi : (bivalC -n> iPropG lang Σ) -n> (bivalC -n> iPropG lang Σ)) :
-    Contractive (interp_rec_pre τi).
+  Global Instance interp_var_persistent τ Δ vv :
+    ctx_PersistentP Δ → PersistentP (interp τ Δ vv).
   Proof.
-    intros n f g H w; cbn.
-    apply always_ne, exist_ne; intros e; apply and_ne; trivial.
-    apply later_contractive =>i Hi. rewrite H; trivial.
+    revert vv Δ; induction τ=> vv Δ HΔ; simpl; try apply _.
+    rewrite /PersistentP /interp_rec fixpoint_unfold /interp_rec1 /=.
+    by apply always_intro'.
   Qed.
 
-  Program Definition interp_rec :
-      ((bivalC -n> iPropG lang Σ) -n> (bivalC -n> iPropG lang Σ)) -n>
-      (bivalC -n> iPropG lang Σ) := λne τi,
-    fixpoint (interp_rec_pre τi).
-  Next Obligation. intros n f g H; apply fixpoint_ne => z; rewrite H; trivial. Qed.
-
-  Context `{i : heapIG Σ} (L : namespace).
-
-  Program Definition interp_ref_pred (l : loc * loc) :
-      (bivalC -n> iPropG lang Σ) -n> iPropG lang Σ := λne τi,
-    (∃ v, (l.1) ↦ᵢ (v.1) ★ (l.2) ↦ₛ (v.2) ★ (τi v))%I.
-  Next Obligation. solve_proper. Qed.
-
-  Program Definition interp_ref :
-      (bivalC -n> iPropG lang Σ) -n> bivalC -n> iPropG lang Σ := λne τi w,
-    (∃ l, w = (LocV (l.1), LocV (l.2)) ∧ inv (L .@ l) (interp_ref_pred l τi))%I.
-  Next Obligation.
-    intros τi n [x1 x2] [y1 y2] [H1 H2]; simpl in *.
-    inversion H1; inversion H2; subst; trivial.
-  Qed.
-  Next Obligation. solve_proper. Qed.
-
-  Program Fixpoint interp (τ : type) {struct τ} :
-      (varC -n> bivalC -n> iPropG lang Σ) -n> bivalC -n> iPropG lang Σ :=
-    match τ return (varC -n> bivalC -n> iPropG lang Σ) -n>
-                   bivalC -n> iPropG lang Σ with
-    | TUnit => λne Δ, interp_unit
-    | TNat => λne Δ, interp_nat
-    | TBool => λne Δ, interp_bool
-    | TProd τ1 τ2 => λne Δ, interp_prod (interp τ1 Δ) (interp τ2 Δ)
-    | TSum τ1 τ2 => λne Δ, interp_sum(interp τ1 Δ) (interp τ2 Δ)
-    | TArrow τ1 τ2 => λne Δ, interp_arrow (interp τ1 Δ) (interp τ2 Δ)
-    | TVar v => λne Δ, (Δ v)
-    | TForall τ' =>λne Δ, interp_forall  (extend_context_interp_apply Δ (interp τ'))
-    | TRec τ' => λne Δ, interp_rec (extend_context_interp_apply Δ (interp τ'))
-    | Tref τ' => λne Δ, interp_ref (interp τ' Δ)
-    end%I.
-  Solve Obligations
-  with repeat intros ?;
-              match goal with [H : _ ≡{_}≡ _|- _] => rewrite H end; trivial.
-
-  Global Instance interp_Persistent
-      τ (Δ : varC -n> bivalC -n> iPropG lang Σ)
-      {HΔ : ∀ x vw, PersistentP (Δ x vw)} :
-    ∀ vw, PersistentP (interp τ Δ vw).
+  Lemma interp_weaken Δ1 Π Δ2 τ :
+    interp τ.[iter (length Δ1) up (ren (+ length Π))] (Δ1 ++ Π ++ Δ2)
+    ≡ interp τ (Δ1 ++ Δ2).
   Proof.
-    revert Δ HΔ.
-    induction τ; cbn; intros Δ HΔ v; try apply _.
-    rewrite /PersistentP /interp_rec fixpoint_unfold /interp_rec_pre; cbn.
-    apply always_intro'; trivial.
+    revert Δ1 Π Δ2. induction τ=> Δ1 Π Δ2; simpl; auto.
+    - intros ww; simpl; properness; auto.
+    - intros ww; simpl; properness; auto.
+    - intros ww; simpl; properness; auto.
+    - intros ww; simpl; properness; auto. by apply IHτ1. by apply IHτ2.
+    - intros ww; simpl; properness; auto. by apply IHτ1. by apply IHτ2.
+    - intros ww; simpl; properness; auto. by apply IHτ1. by apply IHτ2.
+    - apply fixpoint_proper=> τi ww /=.
+      properness; auto. apply (IHτ (_ :: _)).
+    - rewrite iter_up; destruct lt_dec as [Hl | Hl]; simpl.
+      { by rewrite !lookup_app_l. }
+      change (uPredC (iResUR lang _)) with (iPropG lang Σ).
+      rewrite !lookup_app_r; [|lia ..]. do 2 f_equiv. lia. done.
+    - intros ww; simpl; properness; auto. by apply (IHτ (_ :: _)).
+    - intros ww; simpl; properness; auto. by apply IHτ.
   Qed.
 
-  Global Instance extend_context_interp_Persistent
-    (f : bivalC -n> iPropG lang Σ) (Δ : varC -n> bivalC -n> iPropG lang Σ)
-           (Hf : ∀ vw, PersistentP (f vw))
-           {HΔ : ∀ x vw, PersistentP (Δ x vw)}
-    : ∀ x vw, PersistentP (@extend_context_interp f Δ x vw).
-  Proof. intros x v. destruct x; cbn; trivial. Qed.
-
-  Local Ltac properness :=
-    repeat
-      match goal with
-      | |- (∃ _: _, _)%I ≡ (∃ _: _, _)%I => apply exist_proper =>?
-      | |- (∀ _: _, _)%I ≡ (∀ _: _, _)%I => apply forall_proper =>?
-      | |- (_ ∧ _)%I ≡ (_ ∧ _)%I => apply and_proper
-      | |- (_ ∨ _)%I ≡ (_ ∨ _)%I => apply or_proper
-      | |- (_ → _)%I ≡ (_ → _)%I => apply impl_proper
-      | |- (WP _ {{ _ }})%I ≡ (WP _ {{ _ }})%I => apply wp_proper =>?
-      | |- (▷ _)%I ≡ (▷ _)%I => apply later_proper
-      | |- (□ _)%I ≡ (□ _)%I => apply always_proper
-      | |- (inv _ _)%I ≡ (inv _ _)%I => apply (contractive_proper _)
-      | |- (_ ★ _)%I ≡ (_ ★ _)%I => apply sep_proper
-      end.
-
-  Lemma interp_unused_contex_irrel
-        (m n : nat)
-        (Δ Δ' : varC -n> bivalC -n> iPropG lang Σ)
-        (HΔ : ∀ v, Δ (if lt_dec v m then v else (n + v)) ≡
-                     Δ' (if lt_dec v m then v else (n + v)))
-        (τ : type)
-    :
-      interp τ.[iter m up (ren (+n))] Δ ≡ interp τ.[iter m up (ren (+n))] Δ'.
+  Lemma interp_subst_up Δ1 Δ2 τ τ' :
+    interp τ (Δ1 ++ interp τ' Δ2 :: Δ2)
+    ≡ interp τ.[iter (length Δ1) up (τ' .: ids)] (Δ1 ++ Δ2).
   Proof.
-    revert m n Δ Δ' HΔ.
-    induction τ; intros m n Δ Δ' HΔ v; cbn; auto.
-    - properness; trivial; try apply IHτ1; try apply IHτ2; trivial.
-    - properness; trivial; try apply IHτ1; try apply IHτ2; trivial.
-    - properness; trivial; try apply IHτ1; try apply IHτ2; trivial.
-    - match goal with
-        |- _ _ ?f ?x ≡ _ _ ?g ?x =>
-        assert (f ≡ g) as Hfg; [|rewrite Hfg; trivial]
-      end.
-      apply fixpoint_proper => ??; cbn.
-      properness; trivial.
-      change (up (iter m up (ren (+n)))) with (iter (S m) up (ren (+n))).
-      apply IHτ.
-      {
-        intros x y. destruct x; cbn; trivial.
-        destruct lt_dec.
-        - specialize (HΔ x); destruct lt_dec; auto with omega.
-        - destruct (n + S x) as [|k] eqn:Heq; trivial.
-          specialize (HΔ x); destruct lt_dec; auto with omega.
-          replace (n + x) with k in HΔ by omega; trivial.
-      }
-    -  rewrite iter_up. destruct lt_dec; cbn.
-       + specialize (HΔ x); destruct lt_dec; auto with omega.
-       + asimpl; unfold ids; cbn.
-         specialize (HΔ x); destruct lt_dec; auto with omega.
-         replace (m + n + (x - m)) with (n + x) by omega. trivial.
-    - properness; trivial.
-      change (up (iter m up (ren (+n)))) with (iter (S m) up (ren (+n))).
-      apply IHτ.
-      {
-        intros x y. destruct x; cbn; trivial.
-        destruct lt_dec.
-        - specialize (HΔ x); destruct lt_dec; auto with omega.
-        - destruct (n + S x) as [|k] eqn:Heq; trivial.
-          specialize (HΔ x); destruct lt_dec; auto with omega.
-          replace (n + x) with k in HΔ by omega; trivial.
-      }
-    - properness; trivial; try apply IHτ; trivial.
+    revert Δ1 Δ2; induction τ=> Δ1 Δ2; simpl; auto.
+    - intros ww; simpl; properness; auto.
+    - intros ww; simpl; properness; auto.
+    - intros ww; simpl; properness; auto.
+    - intros ww; simpl; properness; auto. by apply IHτ1. by apply IHτ2.
+    - intros ww; simpl; properness; auto. by apply IHτ1. by apply IHτ2.
+    - intros ww; simpl; properness; auto. by apply IHτ1. by apply IHτ2.
+    - apply fixpoint_proper=> τi ww /=.
+      properness; auto. apply (IHτ (_ :: _)).
+    - rewrite iter_up; destruct lt_dec as [Hl | Hl]; simpl.
+      { by rewrite !lookup_app_l. }
+      change (uPredC (iResUR lang _)) with (iPropG lang Σ).
+      rewrite !lookup_app_r; [|lia ..].
+      destruct (x - length Δ1) as [|n] eqn:?; simpl.
+      { symmetry. asimpl. apply (interp_weaken [] Δ1 Δ2 τ'). }
+      change (uPredC (iResUR lang _)) with (iPropG lang Σ).
+      rewrite !lookup_app_r; [|lia ..]. do 2 f_equiv. lia. done.
+    - intros ww; simpl; properness; auto. apply (IHτ (_ :: _)).
+    - intros ww; simpl; properness; auto. by apply IHτ.
   Qed.
 
-  Program Definition hop_context_interp (m n : nat) :
-      (varC -n> bivalC -n> iPropG lang Σ) -n>
-      (varC -n> bivalC -n> iPropG lang Σ) := λne Δ v,
-    if lt_dec v m then Δ v else Δ (v - n).
-  Next Obligation. intros ?????? Hxy; destruct Hxy; trivial. Qed.
-  Next Obligation.
-    intros ????? Hfg ?; cbn. destruct lt_dec; rewrite Hfg; trivial.
-  Qed.
+  Lemma interp_subst Δ2 τ τ' : interp τ (interp τ' Δ2 :: Δ2) ≡ interp τ.[τ'/] Δ2.
+  Proof. apply (interp_subst_up []). Qed.
 
-  Lemma extend_bofore_hop_context_interp (m n : nat)
-      (Δ : varC -n> bivalC -n> iPropG lang Σ)
-      (τi : bivalC -n> iPropG lang Σ) (v : var) :
-    extend_context_interp τi (hop_context_interp m n Δ)
-                             (if lt_dec v (S m) then v else n + v)
-    ≡ hop_context_interp (S m) n (extend_context_interp τi Δ)
-                                 (if lt_dec v (S m) then v else n + v).
+  Lemma context_interp_ren_S Δ (Γ : list type) (vvs : list (val * val)) τi :
+    ([∧] zip_with (λ τ, interp τ Δ) Γ vvs)
+    ⊣⊢ ([∧] zip_with (λ τ, interp τ.[ren (+1)] (τi :: Δ)) Γ vvs).
   Proof.
-    destruct v; cbn; trivial.
-    repeat (destruct lt_dec; cbn); auto with omega.
-    destruct (n + S v - n) eqn:Heq1;
-      destruct (n + S v) eqn:Heq2; try destruct lt_dec; auto with omega.
-    match goal with
-      [ |- _ _ _ Δ ?a ≡ _ _ _ Δ ?b] => assert (Heq : a = b) by omega;
-                                       rewrite Heq; trivial
-    end.
+    revert Δ vvs τi; induction Γ=> Δ [|vv vvs] τi; simpl; auto.
+    apply and_proper; auto.
+    symmetry. apply (interp_weaken [] [τi] Δ).
   Qed.
 
-  Lemma interp_subst_weaken
-      (m n : nat) (Δ : varC -n> bivalC -n> iPropG lang Σ) (τ : type) :
-    interp τ Δ ≡ interp τ.[iter m up (ren (+n))] (hop_context_interp m n Δ).
+  Lemma interp_EqType_agree τ v v' Δ :
+    ctx_PersistentP Δ → EqType τ → interp τ Δ (v, v') ⊢ ■ (v = v').
   Proof.
-    revert m n Δ.
-    induction τ; intros m n Δ v; cbn -[extend_context_interp]; auto.
-    - properness; trivial; try apply IHτ1; try apply IHτ2.
-    - properness; trivial; try apply IHτ1; try apply IHτ2.
-    - properness; trivial; try apply IHτ1; try apply IHτ2.
-    - match goal with
-        |- _ _ ?f ?x ≡ _ _ ?g ?x =>
-        assert (f ≡ g) as Hfg; [|rewrite Hfg; trivial]
-      end.
-      apply fixpoint_proper => ??; cbn -[extend_context_interp].
-      properness; trivial.
-      rewrite IHτ.
-      change (up (iter m up (ren (+n)))) with (iter (S m) up (ren (+n))).
-      apply interp_unused_contex_irrel.
-      intros w; rewrite extend_bofore_hop_context_interp; trivial.
-    - rewrite iter_up.
-      asimpl; unfold ids; cbn; destruct lt_dec; cbn; destruct lt_dec; auto with omega.
-      replace (m + n + (x - m)) with (x + n) by omega.
-      replace (x + n - n) with x; trivial.
-      { unfold var in *; omega. }
-    - properness; trivial.
-      change (up (iter m up (ren (+n)))) with (iter (S m) up (ren (+n))).
-      rewrite IHτ.
-      apply interp_unused_contex_irrel.
-      intros w; rewrite extend_bofore_hop_context_interp; trivial.
-    - properness; trivial; try apply IHτ; trivial.
-  Qed.
-
-  Lemma interp_ren_S (τ : type)
-      (Δ : varC -n> bivalC -n> iPropG lang Σ) (τi : bivalC -n> iPropG lang Σ) :
-    interp τ Δ ≡ interp τ.[ren (+1)] (extend_context_interp τi Δ).
-  Proof.
-    rewrite (interp_subst_weaken 0 1).
-    apply interp_unused_contex_irrel.
-    clear. intros [|v]; cbn; trivial.
-  Qed.
-
-  Local Opaque eq_nat_dec.
-
-  Program Definition context_interp_insert (m : nat) :
-      (bivalC -n> iPropG lang Σ) -n>
-      (varC -n> bivalC -n> iPropG lang Σ) -n>
-      (varC -n> bivalC -n> iPropG lang Σ) := λne τi Δ v,
-    if lt_dec v m then Δ v else if eq_nat_dec v m then τi else Δ (v - 1).
-  Next Obligation. intros m τi Δ n x y Hxy; destruct Hxy; trivial. Qed.
-  Next Obligation.
-    intros m τi n Δ Δ' HΔ x; cbn;
-      destruct lt_dec; try destruct eq_nat_dec; auto.
-  Qed.
-  Next Obligation.
-    intros m n f g Hfg F Δ x; cbn;
-      destruct lt_dec; try destruct eq_nat_dec; auto.
-  Qed.
-
-  Lemma extend_context_interp_insert (m : nat)
-      (τi : bivalC -n> iPropG lang Σ)
-      (Δ : varC -n> bivalC -n> iPropG lang Σ)
-      (Ti : bivalC -n> iPropG lang Σ) :
-    extend_context_interp Ti (context_interp_insert m τi Δ)
-    ≡ context_interp_insert (S m) τi (extend_context_interp Ti Δ).
-  Proof.
-    intros [|v]; cbn; trivial.
-    repeat destruct lt_dec; trivial;
-      repeat destruct eq_nat_dec; cbn; auto with omega.
-    destruct v; cbn; auto with omega.
-    replace (v - 0) with v by omega; trivial.
-  Qed.
-
-  Lemma context_interp_insert_O_extend
-      (τi : bivalC -n> iPropG lang Σ)
-      (Δ : varC -n> bivalC -n> iPropG lang Σ) :
-    context_interp_insert O τi Δ ≡ extend_context_interp τi Δ.
-  Proof.
-    intros [|v]; cbn; trivial.
-    repeat destruct lt_dec; trivial;
-      repeat destruct eq_nat_dec; cbn; auto with omega.
-    destruct v; cbn; auto with omega.
-  Qed.
-
-  Lemma iter_up_subst_type (m : nat) (τ : type) (x : var) :
-    iter m up (τ .: ids) x =
-      if lt_dec x m then ids x else
-        if eq_nat_dec x m then τ.[ren (+m)] else ids (x - 1).
-  Proof.
-    revert x τ.
-    induction m; intros x τ; cbn.
-    - destruct x; cbn.
-      + destruct eq_nat_dec; auto with omega.
-        asimpl; trivial.
-      + destruct eq_nat_dec; auto with omega.
-    - destruct x; asimpl; trivial.
-      rewrite IHm.
-      repeat destruct lt_dec; repeat destruct eq_nat_dec;
-        asimpl; auto with omega.
-  Qed.
-
-  Lemma interp_subst_iter_up
-      (m : nat) (Δ : varC -n> bivalC -n> iPropG lang Σ) (τ τ' : type) :
-    interp τ (context_interp_insert m (interp τ'.[ren (+m)] Δ) Δ)
-    ≡ interp τ.[iter m up (τ' .: ids)] Δ.
-  Proof.
-    revert m Δ.
-    induction τ; intros m Δ v; cbn -[extend_context_interp]; auto.
-    - properness; trivial; try apply IHτ1; try apply IHτ2.
-    - properness; trivial; try apply IHτ1; try apply IHτ2.
-    - properness; trivial; try apply IHτ1; try apply IHτ2.
-    - match goal with
-        |- _ _ ?f ?x ≡ _ _ ?g ?x =>
-        assert (f ≡ g) as Hfg; [|rewrite Hfg; trivial]
-      end.
-      apply fixpoint_proper => ??; cbn -[extend_context_interp].
-      properness; trivial.
-      rewrite extend_context_interp_insert.
-      change (up (iter m up (τ' .: ids))) with (iter (S m) up (τ' .: ids)).
-      rewrite -IHτ.
-      replace (τ'.[ren (+S m)]) with ((τ'.[ren (+m)]).[ren (+1)])
-        by (asimpl; trivial).
-      rewrite -interp_ren_S; trivial.
-    - rewrite iter_up_subst_type.
-      repeat destruct lt_dec; repeat destruct eq_nat_dec;
-        unfold ids; asimpl; trivial.
-    - properness; trivial.
-      rewrite extend_context_interp_insert.
-      change (up (iter m up (τ' .: ids))) with (iter (S m) up (τ' .: ids)).
-      rewrite -IHτ.
-      replace (τ'.[ren (+S m)]) with ((τ'.[ren (+m)]).[ren (+1)])
-        by (asimpl; trivial).
-      rewrite -interp_ren_S; trivial.
-    - properness; trivial; try apply IHτ; trivial.
-  Qed.
-
-  Lemma interp_subst
-      (Δ : varC -n> bivalC -n> iPropG lang Σ) (τ τ' : type) :
-    interp τ (extend_context_interp (interp τ' Δ) Δ) ≡ interp τ.[τ'/] Δ.
-  Proof.
-    rewrite -(interp_subst_iter_up O Δ τ τ').
-    rewrite context_interp_insert_O_extend.
-    asimpl; trivial.
-  Qed.
-
-  Lemma zip_with_context_interp_subst
-      (Δ : varC -n> bivalC -n> iPropG lang Σ) (Γ : list type)
-      (vs : list bivalC) (τi : bivalC -n> iPropG lang Σ) :
-    ([∧] zip_with (λ τ, interp τ Δ) Γ vs)
-    ⊣⊢ ([∧] zip_with (λ τ, interp τ (extend_context_interp τi Δ))
-                     (map (λ t : type, t.[ren (+1)]) Γ) vs).
-  Proof.
-    revert Δ vs τi.
-    induction Γ as [|Γ]; intros Δ vs τi; cbn; trivial.
-    destruct vs; cbn; trivial.
-    apply and_proper. apply interp_ren_S. apply IHΓ.
-  Qed.
-
-  Lemma EqType_related_eq τ {H : EqType τ} v v' (Δ : varC -n> bivalC -n> iPropG lang Σ)
-      {HΔ : ∀ x vw, PersistentP (Δ x vw)} :
-    interp τ Δ (v, v') ⊢ ■ (v = v').
-  Proof.
-    revert v v'; induction H; iIntros {v v'} "#H1 /=".
+    intros ? Hτ; revert v v'; induction Hτ; iIntros {v v'} "#H1 /=".
     - by iDestruct "H1" as "[% %]"; subst.
     - by iDestruct "H1" as {n} "[% %]"; subst.
     - by iDestruct "H1" as {b} "[% %]"; subst.
     - iDestruct "H1" as { [??] [??] } "[% [H1 H2]]"; simplify_eq/=.
-      rewrite IHEqType1 IHEqType2.
+      rewrite IHHτ1 IHHτ2.
       by iDestruct "H1" as "%"; iDestruct "H2" as "%"; subst.
     - iDestruct "H1" as "[H1|H1]".
       + iDestruct "H1" as { [??] } "[% H1]"; simplify_eq/=.
-        rewrite IHEqType1. by iDestruct "H1" as "%"; subst.
+        rewrite IHHτ1. by iDestruct "H1" as "%"; subst.
       + iDestruct "H1" as { [??] } "[% H1]"; simplify_eq/=.
-        rewrite IHEqType2. by iDestruct "H1" as "%"; subst.
+        rewrite IHHτ2. by iDestruct "H1" as "%"; subst.
   Qed.
 End logrel.
